[CBPV] Pull out all reflexive, transitive closures to use a generic RTC

CBPV/CK.lean
@@ -1,3 +1,4 @@
+import CBPV.RTC
 import CBPV.Syntax
 
 inductive F : Type where
@@ -21,25 +22,5 @@ inductive Step : CK → CK → Prop where
 end
 infix:40 "⤳" => Step
 
-/-* Reflexive, transitive closure *-/
-
-inductive RTC {A : Type} (R : A → A → Prop) : A → A → Prop
-  | refl {a} : RTC R a a
-  | trans {a b c} : R a b → RTC R b c → RTC R a c
-infix:40 "⤳⋆"  => RTC Step
-
-def RTC.trans' {A R} {a b c : A} (rab : RTC R a b) (rbc : RTC R b c) : RTC R a c := by
-  induction rab
-  case refl => exact rbc
-  case trans => constructor <;> apply_rules
-
-def RTC.once {A R} {a b : A} (r : R a b) : RTC R a b := .trans r .refl
-
-instance {A} {R : A → A → Prop} : Trans R (RTC R) (RTC R) where
-  trans := .trans
-
-instance {A} {R : A → A → Prop} : Trans R R (RTC R) where
-  trans r₁ r₂ := .trans r₁ (.once r₂)
-
-instance {A} {R : A → A → Prop} : Trans (RTC R) R (RTC R) where
-  trans r₁ r₂ := .trans' r₁ (.once r₂)
+@[reducible] def Steps := RTC Step
+infix:40 "⤳⋆"  => Steps
