CBPV/Evaluation.lean
@@ -1,3 +1,4 @@
+import CBPV.RTC
 import CBPV.Syntax
 
 open Val Com
@@ -37,40 +38,26 @@ theorem evalDet {m n₁ n₂} (r₁ : m ⇒ n₁) (r₂ : m ⇒ n₂) : n₁ = n
   Multi-step evaluation
 ----------------------*-/
 
-section
-set_option hygiene false
-local infix:40 "⇒⋆" => Evals
-inductive Evals : Com → Com → Prop where
-  | refl a : a ⇒⋆ a
-  | trans {a b c} : a ⇒ b → b ⇒⋆ c → a ⇒⋆ c
-end
+@[reducible] def Evals := RTC Eval
 infix:40 "⇒⋆" => Evals
-open Evals
-
-theorem Evals.once {a b} (r : a ⇒ b) : a ⇒⋆ b := .trans r (.refl b)
-
-theorem Evals.trans' {a b c} (r₁ : a ⇒⋆ b) (r₂ : b ⇒⋆ c) : a ⇒⋆ c := by
-  induction r₁ generalizing c
-  case refl => exact r₂
-  case trans r₁ _ ih => exact .trans r₁ (ih r₂)
 
 theorem Evals.app {m n v} (r : m ⇒⋆ n) : app m v ⇒⋆ app n v := by
   induction r
-  case refl => exact .refl _
+  case refl => exact .refl
   case trans r _ ih => exact .trans (.app r) ih
 
 theorem Evals.let {m m' n} (r : m ⇒⋆ m') : letin m n ⇒⋆ letin m' n := by
   induction r
-  case refl => exact .refl _
+  case refl => exact .refl
   case trans r _ ih => exact .trans (.letin r) ih
 
 -- Multi-step reduction is confluent trivially by determinism
 theorem confluence {m n₁ n₂} (r₁ : m ⇒⋆ n₁) (r₂ : m ⇒⋆ n₂) : ∃ m', n₁ ⇒⋆ m' ∧ n₂ ⇒⋆ m' := by
   induction r₁ generalizing n₂
-  case refl => exact ⟨n₂, r₂, refl n₂⟩
+  case refl => exact ⟨n₂, r₂, .refl⟩
   case trans r₁ rs₁ ih =>
     cases r₂
-    case refl => exact ⟨_, refl _, trans r₁ rs₁⟩
+    case refl => exact ⟨_, .refl, .trans r₁ rs₁⟩
     case trans r₂ rs₂ => rw [evalDet r₁ r₂] at *; exact ih rs₂
 
 /-*----------------------------
